template-rocq/theories/LoopChecking/UnivLoopChecking.v
@@ -1,0 +1,300 @@
+(* Distributed under the terms of the MIT license. *)
+(* This module provides an instantiation of the deciders for universe checking,
+  i.e. for constraints on non-empty level expressions (l, k) where k ∈ 𝐍 *)
+
+From Stdlib Require Import ssreflect ssrbool.
+From Stdlib Require Import Program RelationClasses Morphisms.
+From Stdlib Require Import Orders OrderedTypeAlt OrderedTypeEx MSetList MSetInterface MSetAVL MSetFacts FMapInterface MSetProperties MSetDecide.
+From MetaRocq.Utils Require Import utils.
+From MetaRocq.Common Require Import Universes.
+From MetaRocq.Common.LoopChecking Require Import Common Interfaces Deciders.
+From Equations Require Import Equations.
+Set Equations Transparent.
+
+Import Universes.
+
+Module MoreLevel.
+  Import Universes.
+  Include Level.
+
+  Definition to_string := string_of_level.
+End MoreLevel.
+
+Module LevelMap.
+  Module OT := FMapOrderedType_from_UsualOrderedType Level.
+  Include FMapAVL.Make OT.
+End LevelMap.
+
+Module LevelExprZ.
+  Definition t := (Level.t * Z)%type.
+  Local Open Scope Z_scope.
+
+  Definition succ (l : t) : t := (fst l, Z.succ (snd l)).
+
+  Definition eq : t -> t -> Prop := eq.
+
+  Definition eq_equiv : Equivalence eq := _.
+
+  Inductive lt_ : t -> t -> Prop :=
+  | ltLevelExpr1 l n n' : (n < n') -> lt_ (l, n) (l, n')
+  | ltLevelExpr2 l l' b b' : Level.lt l l' -> lt_ (l, b) (l', b').
+  Derive Signature for lt_.
+  Definition lt := lt_.
+
+  Global Instance lt_strorder : StrictOrder lt.
+  Proof.
+    constructor.
+    - intros x X; inversion X. subst. lia. subst.
+      eapply Level.lt_strorder; eassumption.
+    - intros x y z X1 X2; invs X1; invs X2; constructor; tea.
+      etransitivity; tea.
+      etransitivity; tea.
+  Qed.
+
+  Definition lt_compat : Proper (Logic.eq ==> Logic.eq ==> iff) lt.
+    intros x x' H1 y y' H2; now rewrite H1 H2.
+  Qed.
+
+  Definition compare (x y : t) : comparison :=
+    match x, y with
+    | (l1, b1), (l2, b2) =>
+      match Level.compare l1 l2 with
+      | Eq => Z.compare b1 b2
+      | x => x
+      end
+    end.
+
+  Definition compare_spec :
+    forall x y : t, CompareSpec (x = y) (lt x y) (lt y x) (compare x y).
+  Proof.
+    intros [? ?] [? ?]; cbn; repeat constructor.
+    destruct (Level.compare_spec t0 t1); repeat constructor; tas.
+    subst.
+    destruct (Z.compare_spec z z0); repeat constructor; tas. congruence.
+  Qed.
+
+  Global Instance reflect_t : ReflectEq t := reflect_prod _ _ .
+
+  Definition eq_dec : forall (l1 l2 : t), {l1 = l2} + {l1 <> l2} := Classes.eq_dec.
+
+  Definition eq_leibniz (x y : t) : eq x y -> x = y := id.
+
+End LevelExprZ.
+
+Module LevelExprZSet.
+  Include MSetList.MakeWithLeibniz LevelExprZ.
+
+  Definition levels (e : t) :=
+    fold (fun le => LevelSet.add (fst le)) e LevelSet.empty.
+
+  Record nonEmptyLevelExprSet
+    := { t_set : t ;
+         t_ne  : is_empty t_set = false }.
+End LevelExprZSet.
+Module LevelExprZSetFacts := WFactsOn LevelExprZ LevelExprZSet.
+Module LevelExprZSetProp := MSetProperties.OrdProperties LevelExprZSet.
+
+Module LevelSet.
+  Include MakeWithLeibniz Level.
+End LevelSet.
+Module LS <: LevelSets.
+  Module Level := MoreLevel .
+  Module LevelSet := LevelSet.
+  Module LevelExpr := LevelExprZ.
+  Module LevelExprSet := LevelExprZSet.
+  Module LevelMap := LevelMap.
+End LS.
+
+Definition to_levelexprzset (u : LevelExprSet.t) : LS.LevelExprSet.t :=
+  LevelExprSet.fold (fun '(l, k) => LS.LevelExprSet.add (l, Z.of_nat k)) u LS.LevelExprSet.empty.
+
+Lemma to_levelexprzset_spec_1 u :
+  forall l k, LevelExprSet.In (l, k) u -> LevelExprZSet.In (l, Z.of_nat k) (to_levelexprzset u).
+Proof.
+  intros l k.
+  rewrite /to_levelexprzset.
+  apply LevelExprSetProp.fold_rec.
+  - move=> s' hs'; now move=> /hs'.
+  - move=> x a s' s'' hin hnin hadd ih /hadd [].
+    + intros ->. apply LevelExprZSet.add_spec. now left.
+    + intros hin'. destruct x. apply LevelExprZSet.add_spec. now right.
+Qed.
+
+Lemma to_levelexprzset_spec_2 u :
+  forall l k, LevelExprZSet.In (l, k) (to_levelexprzset u) -> LevelExprSet.In (l, Z.to_nat k) u /\ (0 <= k)%Z.
+Proof.
+  intros l k.
+  rewrite /to_levelexprzset.
+  apply LevelExprSetProp.fold_rec.
+  - now move=> s' hs' /LevelExprZSetFacts.empty_iff.
+  - move=> x a s' s'' hin hnin hadd ih.
+    destruct x as [l' k'].
+    rewrite LS.LevelExprSet.add_spec => -[].
+    + intros [= -> eq]. subst k. split. apply hadd. now left. lia.
+    + intros hin'. move: (ih hin') => []; split => //. apply hadd; now right.
+Qed.
+
+Program Definition to_atoms (u : Universe.t) : LevelExprZSet.nonEmptyLevelExprSet :=
+  {| LevelExprZSet.t_set := to_levelexprzset u |}.
+Next Obligation.
+  destruct u. cbn.
+  destruct (LevelExprZSet.is_empty _) eqn:he => //.
+  apply LevelExprZSet.is_empty_spec in he.
+  assert (LevelExprSet.is_empty t_set).
+  apply LevelExprSet.is_empty_spec. intros x hin.
+  destruct x. eapply (he (t, Z.of_nat n)).
+  now apply to_levelexprzset_spec_1.
+  congruence.
+Qed.
+
+Definition from_levelexprzset (u : LS.LevelExprSet.t) : LevelExprSet.t :=
+  LS.LevelExprSet.fold (fun '(l, k) => LevelExprSet.add (l, Z.to_nat k)) u LevelExprSet.empty.
+
+Lemma from_levelexprzset_spec u :
+  forall l k, LevelExprZSet.In (l, k) u -> LevelExprSet.In (l, Z.to_nat k) (from_levelexprzset u).
+Proof.
+  intros l k.
+  rewrite /from_levelexprzset.
+  apply LevelExprZSetProp.P.fold_rec.
+  - now move=> s' hs' /hs'.
+  - move=> x a s' s'' hin hnin hadd ih /hadd [].
+    * intros ->. apply LevelExprSet.add_spec. now left.
+    * intros hin'. destruct x. apply LevelExprSet.add_spec. now right.
+Qed.
+
+Lemma from_levelexprzset_spec_2 u :
+  forall l k, LevelExprSet.In (l, k) (from_levelexprzset u) -> exists z, LevelExprZSet.In (l, z) u /\ k = Z.to_nat z.
+Proof.
+  intros l k.
+  rewrite /from_levelexprzset.
+  apply LevelExprZSetProp.P.fold_rec.
+  - now move=> s' hs' /LevelExprSetFact.empty_iff.
+  - move=> x a s' s'' hin hnin hadd ih.
+    destruct x as [l' k'].
+    rewrite LevelExprSet.add_spec => -[].
+    + intros [= -> eq]. subst k. exists k'. split => //. apply hadd. now left.
+    + intros hin'. move: (ih hin') => [z [hin'' ->]]. exists z. split => //.
+      apply hadd. now right.
+Qed.
+
+Program Definition from_atoms (u : LS.LevelExprSet.nonEmptyLevelExprSet) : Universe.t :=
+  {| LevelExprSet.t_set := from_levelexprzset (LS.LevelExprSet.t_set u) |}.
+Next Obligation.
+  destruct u. cbn.
+  destruct (LevelExprSet.is_empty _) eqn:he => //.
+  apply LevelExprSet.is_empty_spec in he.
+  assert (LevelExprZSet.is_empty t_set).
+  apply LevelExprZSet.is_empty_spec. intros x hin.
+  destruct x. eapply (he (t, Z.to_nat z)).
+  now apply from_levelexprzset_spec.
+  congruence.
+Qed.
+
+
+Module UnivLoopChecking.
+  Module LoopCheck := LoopChecking LS.
+
+  Definition to_constraint (x : UnivConstraint.t) : LoopCheck.constraint :=
+    let '(l, d, r) := x in
+    let '(l, d, r) := match d with
+    | ConstraintType.Eq => (l, LoopCheck.UnivEq, r)
+    | ConstraintType.Le k =>
+      if (k <? 0)%Z then (l, LoopCheck.UnivLe, Universe.add (Z.to_nat (- k)) r)
+      else (Universe.add (Z.to_nat k) l, LoopCheck.UnivLe, r)
+    end
+    in (to_atoms l, d, to_atoms r).
+
+  Module Clauses := LoopCheck.Impl.I.Model.Model.Clauses.Clauses.
+
+  Definition level_constraint_to_constraint (x : LevelConstraint.t) : LoopCheck.constraint :=
+    let '(l, d, r) := x in
+    let '(l, d, r) := match d with
+    | ConstraintType.Eq => (Universe.make' l, LoopCheck.UnivEq, Universe.make' r)
+    | ConstraintType.Le k =>
+      if (k <? 0)%Z then (Universe.make' l, LoopCheck.UnivLe, Universe.make (r, Z.to_nat (-k)))
+      else (Universe.make (l, Z.to_nat k), LoopCheck.UnivLe, Universe.make' r)
+    end
+    in (to_atoms l, d, to_atoms r).
+
+  Record univ_model := {
+    model : LoopCheck.model;
+    constraints : UnivConstraintSet.t;
+    repr_constraints : forall c, UnivConstraintSet.In c constraints <->
+      Clauses.Subset (LoopCheck.to_clauses (to_constraint c)) (LoopCheck.Impl.Abstract.clauses model) }.
+
+  Module C := LoopCheck.Impl.I.Model.Model.Clauses.
+  Import C.
+
+  Lemma exists_to_atoms a u :
+    LevelExprSet.Exists (fun lk : LevelExprSet.elt => a = lk) (to_atoms u) ->
+    Universes.LevelExprSet.Exists (fun lk => a = (fst lk, Z.of_nat (snd lk))) u.
+  Proof.
+    rewrite /to_atoms; cbn; move=> [] [l k] [] hin ->.
+    move/to_levelexprzset_spec_2: hin => [] hin hpos.
+    exists (l, Z.to_nat k). split => //=.
+    rewrite Z2Nat.id //.
+  Qed.
+
+  Lemma exists_to_atoms_2 a (u : Universe.t) :
+    Universes.LevelExprSet.Exists (fun lk => a = lk) u ->
+    LevelExprSet.Exists (fun lk : LevelExprSet.elt => a = (lk.1, Z.to_nat lk.2)) (to_atoms u).
+  Proof.
+    rewrite /to_atoms; cbn; move=> [] [l k] [] hin ->.
+    move/to_levelexprzset_spec_1: hin => hin.
+    exists (l, Z.of_nat k). split => //=.
+    rewrite Nat2Z.id //.
+  Qed.
+
+  Equations? init_model : univ_model :=
+  init_model := {| model := LoopCheck.init_model;
+                   constraints := UnivConstraintSet.empty |}.
+  Proof. split; try ucsets.
+    move=> hyp; apply UnivConstraintSetFact.empty_iff.
+    destruct c as [[l d] r]. destruct d; cbn in hyp.
+    destruct Z.ltb. cbn in hyp.
+    move: hyp. rewrite /Clauses.Subset.
+    rw LoopCheck.clauses_of_le_spec.
+    move=> h.
+    have h' := fun a e => h _ (exists_to_atoms_2 _ _ e).
+    specialize (hyp ()) apply hyp.
+    2:{ }
+    de
+clset.
+
+  (* We ignore errors here, which can happen only if the levels are already declared *)
+  Definition declare_levels (m : univ_model) (l : LevelSet.t) :=
+    LevelSet.fold (fun l m => match LoopCheck.declare_level l m with None => m | Some m => m end) l m.
+
+  Definition enforce_level_constraints (m : univ_model) (l : ConstraintSet.t) :=
+    ConstraintSet.fold (fun c m =>
+      match m with
+      | inl m =>
+        let c := (level_constraint_to_constraint c) in
+        match LoopCheck.enforce c m with
+        | None => (inr (c, None))
+        | Some (inl m) => (inl m)
+        | Some (inr u) => (inr (c, Some u))
+        end
+      | inr err => inr err
+      end) l (inl m).
+
+  Import LoopCheck.Impl.I.Model.Model.Clauses.FLS.
+
+  Definition of_constraint (c : LoopCheck.constraint) : UnivConstraint.t :=
+    let '(l, d, r) := c in
+    let d' := match d with
+      | LoopCheck.UnivLe => ConstraintType.Le 0
+      | LoopCheck.UnivEq => ConstraintType.Eq
+      end
+    in
+    (from_atoms l, d', from_atoms r).
+
+  Definition enforce (c : UnivConstraint.t) (m : univ_model) :=
+    match LoopCheck.enforce (to_constraint c) m with
+    |
+
+
+
+
+
+End UnivLoopChecking.
